Rake and RakeMap cleanups

RakeMap.lean
@@ -39,35 +39,29 @@ def rm_ge2 : RakeMap (λn => 2≤n) := {
 This removes all multiples of a number from the rake.
 - `hx: 0 < x` is necessary because we multiply the delta
   by x in the partition step, and delta=0 gives you a cyclic rake.
-- `h0: ¬ prop 0` is something of a hack: we have to do *something*
-  if every term in the rake is a multiple of x. We can't allow
-  `.ks=[]` because that would make `.term` meaningless. We *could*
-  have `rem` return `Option Rake`, but then you'd have to test for
-  it. Or we could force the callet to provide a proof of
-  `∃m n, r.term m = n ∧ ¬n∣div`
+- `hnmr` is a proof that the rake contains at least one non-multiple of j.
+  This is a number that won't be removed. If all numbers were
+  removed, `term` would become meaningless.
 
--/
-def rem (rm : RakeMap prop) (x: Nat) (hx: 0<x) (h0: ¬prop 0)
-  : RakeMap (λ n => (prop n ∧ ¬(x∣n))) :=
+In the future, it may make sense to also provide a version of
+`rem` that requires no such proof but returns `Option Rake`. -/
+def rem (rm : RakeMap prop) (j: Nat) (hj: 0<j) (hnmr: ∃n m, ¬j∣n ∧ rm.term m = n)
+  : RakeMap (λ n => prop n ∧ ¬j∣n) :=
   let r₀ := rm.rake
-  let r₁ := r₀.rem x hx
-  have hbij₀ := r₀.hbij
-  have hbij₁ : ∀n, (prop n ∧ ¬(x∣n) ↔ ∃ m, r₁.term m = n) := by
+  let r₁ := r₀.rem hj;
+  have hbij₀ := rm.hbij
+  have hbij₁ : ∀n, prop n ∧ ¬j∣n ↔ ∃ m, r₁.term m = n := by
     intro n
-    by_cases hn: 0<n
-    have hb := rm.hbij
-    have hd := r₀.rem_drop x n hx hn
-    have hk := r₀.rem_keep x n hx
-    have ¬∃m, r₀.term m = 0 := by sorry
-    have hs := r₀.rem_same x n hx h0
-    all_goals apply Iff.intro; by_cases x∣n
-    -- aesop can handle 5 of the 6 goals:
-    aesop; aesop; aesop; aesop; aesop
-    -- aesop needs some help with the last case:
-    show (∃ m, r₁.term m = n) → prop n ∧ ¬x ∣ n
-    sorry
+    have hnm: r₀.HasNonMultiple j := by
+      obtain ⟨n, m, hjn, ht⟩ := hnmr
+      dsimp[HasNonMultiple, r₀]
+      use n; aesop
+    have hd := r₀.rem_drop hj
+    have hk := r₀.rem_keep hj
+    have hs := r₀.rem_same hj
+    repeat aesop
   let r₂ := r₁.sort
-  let hbij₂ : ∀ n, prop n ∧ ¬(x∣n) ↔ ∃ m, r₂.val.term m = n := by
+  let hbij₂ : ∀ n, prop n ∧ ¬j∣n ↔ ∃ m, r₂.val.term m = n := by
     intro n
     have hs := r₁.sort_term_iff_term n
     apply Iff.intro; all_goals aesop
